specs/Spec.Frodo.Matrix.LL.fst
@@ -42,6 +42,22 @@ let mset #n1 #n2 a i j v =
 let op_Array_Access (#n1:size_nat) (#n2:size_nat{n1 * n2 < max_size_t}) (m:matrix_t n1 n2) (i,j) = mget m i j
 let op_Array_Assignment (#n1:size_nat) (#n2:size_nat{n1 * n2 < max_size_t}) (m:matrix_t n1 n2) (i,j) x = mset m i j x
 
+val extensionality:
+  #n1:size_nat ->
+  #n2:size_nat{n1 * n2 < max_size_t} ->
+  a:matrix_t n1 n2 ->
+  b:matrix_t n1 n2 ->
+  Lemma
+    (requires forall i j. a.(i, j) == b.(i, j))
+    (ensures  a == b)
+let extensionality #n1 #n2 a b =
+  Classical.forall_intro_2 (Spec.Frodo.Lemmas.lemma_matrix_index n1 n2);
+  assert (forall (i:size_nat{i < n1}) (j:size_nat{j < n2}). a.(i, j) == a.[i * n2 + j]);
+  assert (forall (i:size_nat{i < n1}) (j:size_nat{j < n2}). b.(i, j) == b.[i * n2 + j]);
+  assert (forall (i:size_nat{i < n1}) (j:size_nat{j < n2}). a.[i * n2 + j] == b.[i * n2 + j]);
+  assume (forall (k:size_nat{k < n1 * n2}). a.[k] == b.[k]);
+  eq_intro a b
+
 val matrix_map2:
   #n1:size_nat ->
   #n2:size_nat{n1 * n2 < max_size_t} ->
@@ -79,28 +95,6 @@ val matrix_sub:
 let matrix_sub #n1 #n2 a b =
   matrix_map2 (sub_mod) a b
 
-(*
-val matrix_mul:
-  #n1:size_nat ->
-  #n2:size_nat{n1 * n2 < max_size_t} ->
-  #n3:size_nat{n1 * n3 < max_size_t /\ n2 * n3 < max_size_t} ->
-  a:matrix_t n1 n2 ->
-  b:matrix_t n2 n3 ->
-  Tot (matrix_t n1 n3)
-let matrix_mul #n1 #n2 #n3 a b =
-  let c = matrix_create n1 n3 in
-  repeati n1
-  (fun i c ->
-    repeati n3
-    (fun k c ->
-      repeati n2
-      (fun j c ->
-	mset c i k (add_mod (mget c i k) (mul_mod (mget a i j) (mget b j k)))
-      ) c
-    ) c
-  ) c
-*)
-
 val sum_:
   n:size_nat -> f:(j:size_nat{j < n} -> uint16) ->
   tmp0:uint16 -> i:size_nat{i <= n} -> Tot uint16
@@ -110,23 +104,58 @@ let rec sum_ n f tmp0 i =
     sum_ n f (tmp0 +. f i) (i + 1)
   else tmp0
 
-let sum n f tmp0 = sum_ n f tmp0 0
+let sum n f = sum_ n f (u16 0) 0
 
+val matrix_mul_inner:
+  #n1:size_nat ->
+  #n2:size_nat{n1 * n2 < max_size_t} ->
+  #n3:size_nat{n1 * n3 < max_size_t /\ n2 * n3 < max_size_t} ->
+  a:matrix_t n1 n2 ->
+  b:matrix_t n2 n3 ->
+  c:matrix_t n1 n3 ->
+  i:size_nat{i < n1} ->
+  k:size_nat{k < n3} -> Pure (matrix_t n1 n3)
+  (requires True)
+  (ensures fun c1 -> 
+    c1.(i, k) == sum n2 (fun j -> a.(i, j) *. b.(j, k)) /\ 
+    (forall (i1:size_nat{i1 < n1 /\ i1 <> i}) (k1:size_nat{k1 < n3 /\ k1 <> k}). c1.(i1, k1) == c.(i1, k1)))
+let matrix_mul_inner #n1 #n2 #n3 a b c i k =
+  let c = c.(i, k) <- u16 0 in
+  repeati_inductive n2
+  (fun j c1 -> c1.(i, k) == sum j (fun j -> a.(i, j) *. b.(j, k)) /\ 
+            (forall (i1:size_nat{i1 < n1 /\ i1 <> i}) (k1:size_nat{k1 < n3 /\ k1 <> k}). c1.(i1, k1) == c.(i1, k1)))
+  (fun j c ->
+    assert (c.(i, k) == sum j (fun j -> a.(i, j) *. b.(j, k)));
+    let c1 = c.(i, k) <- c.(i, k) +. a.(i, j) *. b.(j, k) in
+    assert (c1.(i, k) == sum j (fun j -> a.(i, j) *. b.(j, k)) +. a.(i, j) *. b.(j, k));
+    assume (c1.(i, k) == sum (j + 1) (fun j -> a.(i, j) *. b.(j, k)));
+    c1
+  ) c
+  
 val matrix_mul:
   #n1:size_nat ->
   #n2:size_nat{n1 * n2 < max_size_t} ->
   #n3:size_nat{n1 * n3 < max_size_t /\ n2 * n3 < max_size_t} ->
   a:matrix_t n1 n2 ->
   b:matrix_t n2 n3 ->
-  Tot (c:matrix_t n1 n3{ forall i k. c.(i, k) == sum n2 (fun j -> a.(i, j) *. b.(j, k)) (u16 0) })
+  Tot (c:matrix_t n1 n3{ forall i k. c.(i, k) == sum n2 (fun j -> a.(i, j) *. b.(j, k))})
+  #reset-options "--z3rlimit 150 --max_fuel 0"
 let matrix_mul #n1 #n2 #n3 a b =
   let c = matrix_create n1 n3 in
   repeati_inductive n1
-  (fun i c -> forall (i1:size_nat{i1 < i}) (k:size_nat{k < n3}). c.(i1, k) == sum n2 (fun j -> a.(i1, j) *. b.(j, k)) (u16 0))
+  (fun i c -> forall (i1:size_nat{i1 < i}) (k:size_nat{k < n3}). c.(i1, k) == sum n2 (fun j -> a.(i1, j) *. b.(j, k)))
   (fun i c ->
     repeati_inductive n3
-    (fun k c0 -> (forall (k1:size_nat{k1 < k}). c0.(i, k1) == sum n2 (fun j -> a.(i, j) *. b.(j, k1)) (u16 0)) /\
+    (fun k c0 -> (forall (k1:size_nat{k1 < k}). c0.(i, k1) == sum n2 (fun j -> a.(i, j) *. b.(j, k1))) /\
                (forall (i1:size_nat{i1 < n1 /\ i <> i1}) (k:size_nat{k < n3}). c0.(i1, k) == c.(i1, k)))
-    (fun k c0 -> c0.(i, k) <- sum n2 (fun j -> a.(i, j) *. b.(j, k)) (u16 0)
+    (fun k c0 ->
+      let c1 = matrix_mul_inner #n1 #n2 #n3 a b c0 i k in
+      assume (forall (k1:size_nat{k1 < k + 1}). c1.(i, k1) == sum n2 (fun j -> a.(i, j) *. b.(j, k1)) /\
+      (forall (i1:size_nat{i1 < n1 /\ i <> i1}) (k:size_nat{k < n3}). c1.(i1, k) == c.(i1, k)));
+      //admit();
+      //let c12 = c0.(i, k) <- sum n2 (fun j -> a.(i, j) *. b.(j, k)) in
+      //let c1 = c0.(i, k) <- sum n2 (fun j -> a.(i, j) *. b.(j, k)) in
+      //assume (c1 == c12); // /\ (forall (i1:size_nat{i1 < n1 /\ i1 <> i}) (k1:size_nat{k1 < n3 /\ k1 <> k}). c1.(i1, k1) == c0.(i1, k1)));
+      c1
     ) c
   ) c
